

ex 2.4

$f(x, y) = 0$... 関数 (関数)

- (1) $x^2 + y^2 = 4$ の両辺を x で微分する。

$$(x^2)' + \frac{d}{dy} y^2 \cdot \frac{dy}{dx} = (4)'$$

$$2x + 2y y' = 0$$

$$y' = \frac{-2x}{2y} = -\frac{x}{y} \quad \text{①}$$

- (2) 代入 $x = 1 \rightarrow x^2 + y^2 = 4$

$$1^2 + y^2 = 4$$

$$y = \pm\sqrt{3}$$

よって ① より

$$\frac{dy}{dx} \Big|_{(x,y)=(1,\pm\sqrt{3})} = \pm \frac{1}{\sqrt{3}}$$

- 51 (1) 両辺を x で微分する

$$\frac{d}{dy} y^2 \cdot \frac{dy}{dx} = \frac{d}{dy} (4x)$$

$$2y \cdot y' = 4$$

$$y' = \frac{4}{2y} = \frac{2}{y} \quad \text{①}$$

$x = 4$ を与式に代入する

$$y^2 = 4 \cdot 4 = 16$$

$$y = \pm 4$$

① より

$$y' = \frac{4}{2(\pm 4)} = \pm \frac{1}{2}$$

- (2) 与式の両辺を x で微分する

$$(x^2)' + \frac{d}{dy} y^2 \cdot \frac{dy}{dx} = (6)'$$

$$2x + 2y \cdot y' = 0$$

$$y' = \frac{-2x}{2y} = -\frac{x}{y}$$

$x = -1$ を与式に代入する

$$(-1)^2 + y^2 = 6$$

$$y^2 = 5$$

$$y = \pm\sqrt{5}$$

① より

$$y' = -\frac{-1}{\pm\sqrt{5}} = \pm \frac{1}{\sqrt{5}}$$

- 52 (1)

$$y = \frac{4x+1}{(x-2)^{\frac{1}{2}}}$$

$$y' = \frac{(4x+1)'(x-2)^{\frac{1}{2}} - (4x+1) \left\{ (x-2)^{\frac{1}{2}} \right\}'}{\left\{ (x-2)^{\frac{1}{2}} \right\}^2}$$

$$= \frac{4(x-2)^{\frac{1}{2}} - (4x+1) \cdot \frac{1}{2}(x-2)^{-\frac{1}{2}} \cdot 1}{(x-2)}$$

$$= \frac{4(x-2)^{\frac{1}{2}}(x-2) - (4x+1) \cdot \frac{1}{2}(x-2)^{-\frac{1}{2}} \cdot 1}{(x-2)}$$

$$= \frac{4(x-2) - (4x+1) \cdot \frac{1}{2}}{(x-2)(x-2)^{\frac{1}{2}}}$$

$$= \frac{8(x-2) - (4x+1)}{2(x-2)\sqrt{x-2}}$$

$$= \frac{4x-17}{2(x-2)\sqrt{x-2}}$$

- (2) \log の真数 > 0 より $\tan \frac{x}{2} \neq 0$.

$$y' = \frac{1}{\tan \frac{x}{2}} \cdot \left(\tan \frac{x}{2} \right)'$$

$\uparrow \log$ は $\tan \frac{x}{2}$ で微分

$\downarrow \tan \frac{x}{2}$ は $\frac{x}{2}$ で微分

$$= \frac{1}{\frac{\sin \frac{x}{2}}{\cos \frac{x}{2}}} \cdot \frac{1}{\cos^2 \frac{x}{2}} \cdot \frac{1}{2} \leftarrow \frac{x}{2} \text{ は } x \text{ で微分}$$

$$= \frac{1}{2 \sin \frac{x}{2} \cdot \cos \frac{x}{2}}$$

$$\because \text{ここで, } \sin x = \sin \left(\frac{x}{2} + \frac{x}{2} \right)$$

$$= \sin \frac{x}{2} \cos \frac{x}{2} + \cos \frac{x}{2} \sin \frac{x}{2}$$

$$= 2 \sin \frac{x}{2} \cos \frac{x}{2}$$

$$y' = \frac{1}{\sin x}$$

- (3) $y' = \frac{1}{e^x+1} \cdot e^x$

$$= \frac{e^x}{e^x+1}$$

- (4) $y' = (x)' \sin^{-1} \sqrt{x} + x (\sin^{-1} \sqrt{x})'$

$$\because t := \sqrt{x}, \quad g := \sin^{-1} \sqrt{x} = \sin^{-1} t$$

$$\Rightarrow t = \sin g$$

両辺を g で微分する

$$\frac{dt}{dg} = \cos g$$

$$\text{よって } \frac{dy}{dx} = \frac{1}{\frac{dt}{dg}} = \frac{1}{\cos g}$$

$$= \frac{1}{\sqrt{1-\sin^2 g}} \quad \because \sin^2 g + \cos^2 g = 1, \quad -\frac{\pi}{2} \leq g \leq \frac{\pi}{2} \Rightarrow \cos g \geq 0$$

$$= \frac{1}{\sqrt{1-t^2}}$$

よって,

$$(\sin^{-1} \sqrt{x})' = \frac{dg}{dt} \cdot \frac{dt}{dx}$$

$$= \frac{1}{\sqrt{1-t^2}} \cdot \frac{1}{2} x^{-\frac{1}{2}}$$

$$= \frac{1}{2\sqrt{x}\sqrt{1-x}}$$

$$y' = \sin^{-1} \sqrt{x} + \frac{\sqrt{x}}{2\sqrt{x}\sqrt{1-x}}$$

$$= \sin^{-1} \sqrt{x} + \frac{\sqrt{x}}{2\sqrt{1-x}}$$

- (5) $y = \log(x+2)^{\frac{2}{3}}$

$$= \frac{2}{3} \log(x+2)$$

$$y' = \frac{2}{3} \cdot \frac{1}{x+2} \cdot 1$$

$$= \frac{2}{3(x+2)}$$

- 53 (1) $f'(x) = \left(\sqrt{2x^2-x} \right)'$

$$= \left((2x^2-x)^{\frac{1}{2}} \right)'$$

$$= \frac{1}{2} (2x^2-x)^{-\frac{1}{2}} \cdot (2 \cdot 2x - 1)$$

$$= \frac{1}{2} \frac{4x-1}{\sqrt{2x^2-x}}$$

$$= \frac{4x-1}{2\sqrt{2x^2-x}}$$

$$f'(1) = \frac{4 \cdot 1 - 1}{2\sqrt{2 \cdot 1^2 - 1}}$$

$$= \frac{3}{2}$$

- (2) $f'(x) = \cos 3x \cdot 3$

$$= 3 \cos 3x$$

$$f'\left(\frac{7}{3}\pi\right) = 3 \cos\left(3 \cdot \frac{7}{3}\pi\right)$$

$$= 3 \cos 7\pi$$

$$= -3$$

- (3) $f'(x) = \frac{1}{\cos^2 \frac{x}{4}} \cdot \frac{1}{4}$

$$= \frac{1}{4 \cos^2 \frac{x}{4}}$$

$$f'(3\pi) = \frac{1}{4 \cos^2 \frac{3\pi}{4}}$$

$$= \frac{1}{4 \cdot \left(-\frac{1}{\sqrt{2}}\right)^2}$$

$$= \frac{1}{4 \cdot \frac{1}{2}}$$

$$= \frac{1}{2}$$

- (4) $f'(x) = \frac{1}{4x-1} \cdot 4$

$$= \frac{4}{4x-1}$$

$$f'(3) = \frac{4}{4 \cdot 3 - 1}$$

$$= \frac{4}{11}$$

- (5) $f'(x) = (x)'(e^{x^2}) + (x)(e^{x^2})'$

$$= 1 \cdot e^{x^2} + x \cdot e^{x^2} \cdot 2x$$

$$= e^{x^2} (1 + 2x^2)$$

$$f'(2) = e^{2^2} (1 + 2 \cdot 2^2)$$

$$= e^4 (1 + 8)$$

$$= 9e^4$$

- (6) $f'(x) = \frac{(2x+1)'(x-3) - (2x+1)(x-3)'}{(x-3)^2}$

$$= \frac{2(x-3) - (2x+1) \cdot 1}{(x-3)^2}$$

$$= \frac{-7}{(x-3)^2}$$

$$f'(4) = \frac{-7}{(4-3)^2} = -7$$

- 54 (1) $f'(x) = \frac{(2x)'(x^2+1) - (2x)(x^2+1)'}{(x^2+1)^2}$

$$= \frac{2(x^2+1) - 2x(2x)}{(x^2+1)^2}$$

$$= \frac{-2x^2+2}{(x^2+1)^2} = 0$$

$$\because \text{ここで } (x^2+1)^2 \neq 0$$

$$x^2+1 \neq 0$$

$$x^2 \neq -1$$

$$x \neq \pm i$$

$$\frac{-2x^2+2}{(x^2+1)^2} = 0$$

$$-2x^2+2 = 0$$

$$2x^2 = 2$$

$$x^2 = 1$$

$$x = \pm 1$$

- (2) $f'(x) = \frac{(1-x)'(x^2-x+1) - (1-x)(x^2-x+1)'}{(x^2-x+1)^2}$

$$= \frac{-x^2+x-1 - (1-x)(2x-1)}{(x^2-x+1)^2}$$

$$= \frac{-x^2+x-1 - (2x-1-2x^2+x)}{(x^2-x+1)^2}$$

$$= \frac{x^2-2x}{(x^2-x+1)^2} = 0$$

$$\because \text{ここで } x^2-x+1 \neq 0$$

$$x \neq \frac{1 \pm \sqrt{1-4}}{2} = \frac{1 \pm \sqrt{3}i}{2}$$

$$\frac{x^2-2x}{(x^2-x+1)^2} = 0$$

$$x^2-2x = 0$$

$$x(x-2) = 0$$

$$x = 0, 2$$

- 55 (1) $f(x) = 2 \left\{ x(5-x)^{\frac{1}{2}} \right\}'$

$$= 2 \left\{ (x)'(5-x)^{\frac{1}{2}} + x \left\{ (5-x)^{\frac{1}{2}} \right\}' \right\}$$

$$= 2 \left\{ (5-x)^{\frac{1}{2}} + x \cdot \frac{1}{2} (5-x)^{-\frac{1}{2}} \cdot (-1) \right\}$$

$$= 2(5-x)^{\frac{1}{2}} - x(5-x)^{-\frac{1}{2}}$$

$$= 2(5-x)^{\frac{1}{2}} - \frac{x}{\sqrt{5-x}}$$

$$= \frac{2(5-x) - x}{\sqrt{5-x}}$$

$$= \frac{-3x+10}{\sqrt{5-x}} = 0$$

$$\sqrt{5-x} \neq 0 \text{ かつ } -3x+10 \geq 0 \Rightarrow 5-x > 0 \Leftrightarrow x < 5$$

$$\frac{-3x+10}{\sqrt{5-x}} = 0$$

$$-3x+10 = 0$$

$$x = \frac{10}{3}$$

- (2) $f'(x) = \left\{ (x-5)(x^2+3)^{\frac{1}{2}} \right\}'$

$$= (x-5)'(x^2+3)^{\frac{1}{2}} + (x-5) \left\{ (x^2+3)^{\frac{1}{2}} \right\}'$$

$$= 1 \cdot (x^2+3)^{\frac{1}{2}} + (x-5) \cdot \frac{1}{2} (x^2+3)^{-\frac{1}{2}} \cdot 2x$$

$$= (x^2+3)^{\frac{1}{2}} + x(x-5)(x^2+3)^{-\frac{1}{2}}$$

$$= (x^2+3)^{\frac{1}{2}} + \frac{x(x-5)}{(x^2+3)^{\frac{1}{2}}}$$

$$= \frac{x^2+3+x^2-5x}{\sqrt{x^2+3}}$$

$$= \frac{2x^2-5x+3}{\sqrt{x^2+3}}$$

$$= \frac{(2x-3)(x-1)}{\sqrt{x^2+3}} = 0$$

$$\sqrt{x^2+3} \neq 0 \text{ かつ } 2x^2+3 \geq 0 \Rightarrow x^2+3 > 0 \Leftrightarrow x^2 > -3$$

$$(\text{実数})^2 \geq 0 \text{ かつ } -\infty < x < \infty$$

$$\frac{(2x-3)(x-1)}{\sqrt{x^2+3}} = 0$$

$$(2x-3)(x-1) = 0$$

$$x = \frac{3}{2}, 1$$